\documentclass{article}
\newcommand{\beq}{\begin{equation}}
\newcommand{\eeq}{\end{equation}}
\newcommand{\ber}{\begin{eqnarray}}
\newcommand{\eer}{\end{eqnarray}}
\newcommand{\nn}{\nonumber}
\newcommand{\dd}[2]{\frac{d}{d{#2}}{(#1)} }
\usepackage{amsmath}
\usepackage{amsfonts}
\usepackage{url}
\begin{document}
\title{A model to illustrate chain rule for back-propagation}
\author{Nachiket Gokhale}
\date{\today}
\maketitle
\section{Model 1}
Our model is 
\beq
f(x) = g(h(x))
\eeq
where,
\beq
h(x) = a_1x + b_1 \qquad \text{and} \qquad g(x) = a_2x+b_2.
\eeq
We want to estimate the parameters $a_1,b_1,a_2,b_2$. For this we need to differentiate $f$ wrt $a_1,b_1,a_2,b_2$.
\ber
\dd{f}{a_1} &=& \dd{g(u)}{u}\dd{u}{a_1} \qquad \text{ where } u = h(x) = a_1x+b_1 \nn \\
            &=& a_2x \\
\dd{f}{b_1} &=& \dd{g(u)}{u}\dd{u}{b_1} \qquad \text{ where } u = h(x) = a_1x+b_1 \nn \\
&=& a_2 \\
\dd{f}{a_2} &=& \dd{a_2h(x) + b_2}{a_2} = h(x) \\
\dd{f}{b_2} &=& \dd{a_2h(x) + b_2}{b_2} = 1
\eer
\section{Model 2}
Our model is 
\beq
f(x) = g(h(x))
\eeq
where,
\beq
h(x) = \frac{1}{1 + e^{-(a_1x+b_1)}} \qquad \text{and} \qquad g(x) = \frac{1}{1 + e^{-(a_2x+b_2)}}
\eeq
Let
\beq
\sigma(x) = \frac{1}{1+e^{-x}}
\eeq
Then,
\beq
\dd{\sigma(x)}{x} = \sigma(x)(1-\sigma(x))
\eeq
Now,
\ber
\dd{f}{a_1} &=& \dd{g(u)}{u}\dd{u}{a_1} \text{ where } u = h(x) \nn \\
            &=& \dd{\frac{1}{1+e^{-(a_2u+b_2)}}}{u}\dd{\frac{1}{1+e^{-(a_1x+b_1)}}}{a_1} \nn \\
&=& \dd{\frac{1}{1+e^{-(a_2u+b_2)}}}{(a_2u+b_2)}\dd{a_2u+b_2}{u}\dd{\frac{1}{1+e^{-(a_1x+b_1)}}}{((a_1x+b_1))}\dd{a_1x+b_1}{a_1} \nn \\
&=& g(u)(1-g(u))a_2h(x)(1-h(x))x \\
%
\dd{f}{b_1} &=& \dd{g(u)}{u}\dd{u}{b_1} \text{ where } u = h(x) \nn \\
&=& \dd{\frac{1}{1+e^{-(a_2u+b_2)}}}{u}\dd{\frac{1}{1+e^{-(a_1x+b_1)}}}{b_1} \nn \\
&=& g(u)(1-g(u))a_2h(x)(1-h(x)) \\
%
\dd{f}{a_2} &=& \dd{\frac{1}{1+e^{-(a_2u+b_2)}}}{a_2} \text{ where } u = h(x) \nn \\
&=& \dd{\frac{1}{1+e^{-(a_2u+b_2)}}}{(a_2u+b_2)}\dd{a_2u+b_2}{a_2} \nn \\
&=& g(u)(1-g(u))a_2 \\
%
\dd{f}{b_2} &=& \dd{\frac{1}{1+e^{-(a_2u+b_2)}}}{b_2} \text{ where } u = h(x) \nn \\
&=& \dd{\frac{1}{1+e^{-(a_2u+b_2)}}}{(a_2u+b_2)}\dd{a_2u+b_2}{b_2} \nn \\
&=& g(u)(1-g(u))
\eer 
\end{document}
